src/lifting_cont.v
@@ -14,20 +14,26 @@ Fixpoint cont_to_stack k : env_state * nat :=
   | Kseq _ k' | Kwhile _ _ k' => cont_to_stack k'
   end.
 
-Definition stack_match ρ r k := assert_of (λ n, ⌜let '(ρ0, n0) := cont_to_stack k in n = n0 ∧ ρ = <[n := r]>ρ0⌝)%I.
+Definition stack_depth k := snd (cont_to_stack k).
 
-Lemma stack_env_match ρ r k : stack_match ρ r k ⊢ env_match ρ r.
+Definition stack_match ρ r k := let '(ρ0, n) := cont_to_stack k in ρ = <[n := r]>ρ0.
+
+Lemma stack_env_match ρ r k : stack_match ρ r k →
+  stack_level (stack_depth k) ⊢ env_match ρ r.
 Proof.
-  split => n /=; apply bi.pure_mono.
-  destruct (cont_to_stack k); intros (_ & ->); by rewrite lookup_insert.
+  rewrite /stack_level; split => n; monPred.unseal.
+  apply bi.pure_mono; intros <-.
+  unfold stack_match, stack_depth in *.
+  destruct (cont_to_stack k); subst; simpl.
+  by rewrite lookup_insert.
 Qed.
 
-Definition wp_sk_pre (wp : coPset -d> stmt -d> cont -d> assert -d> assert) :
-    coPset -d> stmt -d> cont -d> assert -d> assert := λ E s k Q,
+Definition wp_sk_pre (wp : coPset -d> stmt -d> cont -d> iPropO Σ -d> iPropO Σ) :
+    coPset -d> stmt -d> cont -d> iPropO Σ -d> iPropO Σ := λ E s k Q,
  ((⌜s = Sskip ∧ k = Kstop⌝ ∗ |={E}=> Q) ∨
-  ∀ σ ρ, state_interp σ ρ ={E,∅}=∗ ∀ r, stack_match ρ r k -∗ ∃ s' r' σ' k',
+  ∀ σ ρ, state_interp σ ρ ={E,∅}=∗ ∀ r, ⌜stack_match ρ r k⌝ -∗ ∃ s' r' σ' k',
         ⌜step F s (Build_state r σ k) s' (Build_state r' σ' k')⌝ ∗
-        ▷ |={∅,E}=> ∃ ρ', state_interp σ' ρ' ∗ stack_match ρ' r' k' ∗ wp E s' k' Q)%I.
+        ▷ |={∅,E}=> ∃ ρ', state_interp σ' ρ' ∗ ⌜stack_match ρ' r' k'⌝ ∗ wp E s' k' Q)%I.
 
 Local Instance wp_sk_pre_contractive : Contractive (wp_sk_pre).
 Proof.
@@ -37,12 +43,14 @@ Qed.
 
 Local Definition wp_sk_def := fixpoint wp_sk_pre.
 Local Definition wp_sk_aux : seal (@wp_sk_def). Proof. by eexists. Qed.
-Definition wp_sk := wp_sk_aux.(unseal).
-Local Lemma wp_sk_unseal   : wp_sk = @wp_sk_def.
+Definition wp_sk' := wp_sk_aux.(unseal).
+Local Lemma wp_sk_unseal   : wp_sk' = @wp_sk_def.
 Proof. rewrite -wp_sk_aux.(seal_eq) //. Qed.
 
-Lemma wp_sk_unfold E s k Q : wp_sk E s k Q ⊣⊢ wp_sk_pre wp_sk E s k Q.
+Lemma wp_sk_unfold E s k Q : wp_sk' E s k Q ⊣⊢ wp_sk_pre wp_sk' E s k Q.
 Proof. rewrite wp_sk_unseal. apply (fixpoint_unfold wp_sk_pre). Qed.
+
+Definition wp_sk E s k Q : assert := (stack_level (stack_depth k) -∗ ⎡wp_sk' E s k Q⎤)%I.
 
 Record postassert :=
   { Qnormal : assert; Qbreak : assert; Qcontinue : assert; Qreturn : val → assert }.
@@ -60,43 +68,51 @@ Proof.
   iIntros "H %% Hguard"; by iApply "Hguard".
 Qed.
 
-Lemma var_e : forall x v σ ρ r k, points_to_var x v ∗ state_interp σ ρ ∗ stack_match ρ r k ⊢ ⌜r !! x = Some v⌝.
+Lemma var_e : forall x v σ ρ r k, stack_match ρ r k →
+  stack_level (stack_depth k) ∗ points_to_var x v ∗ ⎡state_interp σ ρ⎤ ⊢ ⌜r !! x = Some v⌝.
 Proof.
-  intros; rewrite /state_interp; split => n; monPred.unseal.
-  iIntros "(Hx & (_ & Hρ) & Hmatch)".
-  iDestruct (var_e with "[$Hx $Hρ]") as %?.
-  destruct (cont_to_stack k) eqn: Hk; iDestruct "Hmatch" as %(<- & ->).
-  by rewrite /env_to_environ lookup_insert in H.
+  intros; rewrite /stack_level; split => n; monPred.unseal.
+  iIntros "(<- & Hx & (_ & Hρ))".
+  iDestruct (var_e with "[$Hx $Hρ]") as %Hr.
+  unfold stack_match, stack_depth in *.
+  destruct (cont_to_stack k) eqn: Hk; subst.
+  by rewrite /env_to_environ lookup_insert in Hr.
 Qed.
 
-Lemma var_update : forall x v v' σ ρ r k, points_to_var x v ∗ state_interp σ ρ ∗ stack_match ρ r k ⊢
-  |==> ∃ ρ', points_to_var x v' ∗ state_interp σ ρ' ∗ stack_match ρ' (<[x := v']>r) k.
+Lemma var_update : forall x v v' σ ρ r k, stack_match ρ r k →
+  stack_level (stack_depth k) ∗ points_to_var x v ∗ ⎡state_interp σ ρ⎤ ⊢
+  |==> ∃ ρ', ⌜stack_match ρ' (<[x := v']>r) k⌝ ∧ points_to_var x v' ∗ ⎡state_interp σ ρ'⎤.
 Proof.
-  intros; rewrite /state_interp; split => n; monPred.unseal.
-  iIntros "(Hx & ($ & Hρ) & Hmatch)".
+  intros; rewrite /stack_level; split => n; monPred.unseal.
+  iIntros "(%Hl & Hx & ($ & Hρ))"; hnf in Hl; subst.
   iMod (var_update with "[$Hx $Hρ]") as "($ & $)".
-  iModIntro; iStopProof; apply bi.pure_mono.
-  destruct (cont_to_stack k) eqn: Hk; intros (<- & ->).
+  iPureIntro.
+  unfold stack_match, stack_depth in *.
+  destruct (cont_to_stack k) eqn: Hk; subst.
   rewrite /set_var lookup_insert insert_insert //.
 Qed.
 
 Lemma wp_assign E x e Q : wp_expr E e (λ v, (∃ v0, points_to_var x v0) ∗
   ▷ (points_to_var x v -∗ Qnormal Q)) ⊢ wp E (Sassign x e) Q.
 Proof.
-  iIntros "H %% Hguard".
+  iIntros "H %% Hguard #Hl".
   rewrite wp_sk_unfold /wp_sk_pre; iRight.
   iIntros (??) "S".
   rewrite /wp_expr.
   iMod ("H" with "S") as (?) "(He & S & (% & Hx) & Hpost)".
-  iApply fupd_mask_intro; first set_solver; iIntros "Hclose" (?) "Hstack".
-  iDestruct (var_e with "[$Hx $S $Hstack]") as %?.
-  iDestruct ("He" with "[Hstack]") as %?; first by iApply stack_env_match.
+  rewrite embed_fupd.
+  iApply fupd_mask_intro; first set_solver; iIntros "Hclose" (? Hstack).
+  iDestruct (var_e with "[$Hl $Hx $S]") as %?; first done.
+  iDestruct ("He" with "[Hl]") as %?; first by iApply stack_env_match.
   iExists _, _, _, _; iSplit.
   { iPureIntro; by constructor. }
   iNext.
-  iMod (var_update with "[$Hx $S $Hstack]") as (?) "(Hx & $ & $)".
+  rewrite embed_fupd.
+  iMod (var_update with "[$Hl $Hx $S]") as (??) "(Hx & $)"; first done.
   iMod "Hclose"; iModIntro.
-  by iApply "Hguard"; iApply "Hpost".
+  iSplit; first done.
+  iDestruct "Hguard" as "(Hguard & _)"; iApply ("Hguard" with "[-] Hl").
+  by iApply "Hpost".
 Qed.
 
 Lemma wp_alloc E x Q : (∃ v0, points_to_var x v0) ∗
@@ -296,7 +312,73 @@ Proof.
   by iApply stack_match_loop'.
 Qed.
 
-(*Lemma wp_call E x f es Q :*)
+Definition get_params f := let 'Func params _ _ := f in params.
+Definition get_locals f := let 'Func _ locals _ := f in locals.
+Definition get_body f := let 'Func _ _ body := f in body.
+
+Definition stack_size f := let 'Func params locals _ := f in
+  (length params + length locals)%nat.
+
+Definition stack_frac f := (/ pos_to_Qp (Pos.of_nat (1 + stack_size f)))%Qp.
+
+Definition stack_retainer f := assert_of (λ n,
+  stack_frag n (stack_frac f) (stack_frac f) ∅).
+
+Definition stackframe f vs := (([∗ list] x;v ∈ (get_params f);vs, points_to_var x v) ∗
+  ([∗ list] x ∈ get_locals f, points_to_var x (NumV 0)))%I.
+
+Definition ret_assert R :=
+  {| Qnormal := False%I; Qbreak := False%I; Qcontinue := False%I; Qreturn := R |}.
+
+Definition call_assert E f vs x R := (⇑ (stack_retainer f -∗ stackframe f vs -∗
+  wp E (get_body f) (ret_assert (λ v, stack_retainer f ∗ (∃ vs, stackframe f vs) ∗
+    ⇓ (points_to_var x v ∗ ▷ (points_to_var x v -∗ R))))))%I.
+
+Lemma wp_exprs_app E es Q σ ρ : wp_exprs E es Q -∗ state_interp σ ρ ={E}=∗
+  ∃ vs, (∀ r k, env_match ρ r -∗ ⌜eval_exprs' es (Build_state r σ k) vs⌝) ∗ state_interp σ ρ ∗ Q vs.
+Proof.
+  iIntros "Hes S"; iInduction es as [|e es] "IH" forall (Q); simpl.
+  - iFrame. iIntros "!> %% ?"; iPureIntro; constructor.
+  - rewrite /wp_expr.
+    iMod ("Hes" with "S") as (?) "(He & S & Hes)".
+    iMod ("IH" with "Hes S") as (?) "(Hes & $ & $)".
+    iIntros "!> %% Henv".
+    iDestruct ("He" with "Henv") as %?; iDestruct ("Hes" $! _ k with "Henv") as %?.
+    iPureIntro; by constructor.
+Qed.
+
+(*Lemma add_frame : forall σ ρ r k x xs vs, state_interp σ ρ ∗ stack_match ρ r k ⊢
+  |==> ∃ ρ', state_interp σ ρ' ∗ stack_match ρ' (bind_vars r xs vs) (Kcall x r k).
+Proof.
+  intros; rewrite /state_interp; split => n; monPred.unseal.
+  iIntros "(($ & Hρ) & %Hρ)".
+  destruct (cont_to_stack k) eqn: Hk; destruct Hρ; subst.
+  iMod (env_alloc with "Hρ").
+  iMod (var_update with "[$Hx $Hρ]") as "($ & $)".
+  iModIntro; iStopProof; apply bi.pure_mono.
+  destruct (cont_to_stack k) eqn: Hk; intros (<- & ->).
+  rewrite /set_var lookup_insert insert_insert //.
+Qed.*)
+
+Lemma wp_call E x f es Q : wp_exprs E es (λ vs, ∃ fd, ⌜F !! f = Some fd ∧ length es = length (get_params fd)⌝ ∧
+  ▷ call_assert E fd vs x (Qnormal Q)) ⊢ wp E (Scall x f es) Q.
+Proof.
+  iIntros "H %% Hguard".
+  rewrite wp_sk_unfold /wp_sk_pre; iRight.
+  iIntros (??) "S".
+  iMod (wp_exprs_app with "H S") as (?) "(Hes & S & %fd & (% & %) & H)".
+  destruct fd; simpl in *.
+  iApply fupd_mask_intro; first set_solver; iIntros "Hclose" (?) "Hstack".
+  iDestruct ("Hes" with "[Hstack]") as %?; first by iApply stack_env_match.
+  iExists _, _, _, _; iSplit.
+  { iPureIntro; by econstructor. }
+  simpl.
+  iNext; iFrame.
+  iMod "Hclose" as "_"; iModIntro; simpl.
+
+  by iApply "H".
+
+Qed.
 
 Lemma find_call_idem k k' : find_call k = Some k' → find_call k' = Some k'.
 Proof.
