src/state_interp.v
@@ -2,28 +2,28 @@ From iris.base_logic Require Export gen_heap.
 From iris_simp_lang Require Import implang_expr.
 From iris_simp_lang Require Export stack_ra.
 
-Notation "l ↦ v" := (⎡pointsto l (DfracOwn 1) v⎤)%I (at level 20).
+Notation "l ↦ v" := (⎡pointsto l (DfracOwn 1) v⎤ : assert)%I (at level 20).
 
 Section state_interp.
 
 Context `{!gen_heapGS loc val Σ} `{!envGS val Σ}.
 
-Definition state_interp σ ρ : assert := (⎡gen_heap_interp σ⎤ ∗ ⎡env_auth ρ⎤)%I.
+Definition state_interp σ ρ : iProp Σ := (gen_heap_interp σ ∗ env_auth ρ)%I.
 
 Lemma state_interp_alloc σ ρ l v : σ !! l = None →
- state_interp σ ρ ==∗ state_interp (<[l := v]>σ) ρ ∗ l ↦ v.
+ ⎡state_interp σ ρ⎤ ==∗ ⎡state_interp (<[l := v]>σ) ρ⎤ ∗ l ↦ v.
 Proof.
   intros; iIntros "(? & $)".
   by iMod (gen_heap_alloc with "[$]") as "($ & $ & _)".
 Qed.
 
-Lemma state_interp_load σ ρ l v : state_interp σ ρ -∗ l ↦ v -∗ ⌜σ !! l = Some v⌝.
+Lemma state_interp_load σ ρ l v : ⎡state_interp σ ρ⎤ -∗ l ↦ v -∗ ⌜σ !! l = Some v⌝.
 Proof.
   by iIntros "(? & _) ?"; iDestruct (gen_heap_valid with "[$] [$]") as %?.
 Qed.
 
-Lemma state_interp_store σ ρ l v v' : state_interp σ ρ -∗ l ↦ v ==∗
-  state_interp (<[l := v']>σ) ρ ∗ l ↦ v'.
+Lemma state_interp_store σ ρ l v v' : ⎡state_interp σ ρ⎤ -∗ l ↦ v ==∗
+  ⎡state_interp (<[l := v']>σ) ρ⎤ ∗ l ↦ v'.
 Proof.
   by iIntros "(? & $) ?"; iMod (gen_heap_update with "[$] [$]") as "($ & $)".
 Qed.
