src/implang.v
@@ -24,7 +24,7 @@ Inductive stmt :=
 .
 
 Inductive func :=
-  | Func (func_params : list string) (func_body : stmt).
+  | Func (func_params : list string) (func_locals : list string) (func_body : stmt).
 
 Bind Scope stmt_scope with stmt.
 Bind Scope func_scope with func.
@@ -103,11 +103,11 @@ Inductive step : func_env -> stmt → state → stmt → state → Prop :=
   | WhileS F e s σ v :
     eval_expr' e σ (NumV v) →
     step F (Swhile e s) σ (if Z.eqb v 0 then Sskip else Sseq s (Swhile e s)) σ
-  | CallS F f es σ ps s vs rv :
-    F !! f = Some (Func ps s) →
+  | CallS F f es σ ps ls s vs rv :
+    F !! f = Some (Func ps ls s) →
     length ps = length es →
     eval_exprs' es σ vs →
-    let ρ' := bind_vars σ.(ρ) ps vs in
+    let ρ' := bind_vars σ.(ρ) (ps ++ ls) (vs ++ repeat (NumV 0) (length ls)) in
     let k' := ((σ.(ρ), rv) :: σ.(k)) in
     step F (Scall rv f es) σ s 
                 (σ <| ρ := ρ' |> <| k:=k' |>)
